Use [nd_seqs] for [wp_args].
Remove [vararg_promote].
Eliminate [wp_call_initialize].

theories/lang/cpp/logic/wp.v
@@ -263,19 +263,46 @@ Section with_cpp.
   Definition Mrel T : M T -> M T -> Prop :=
     (pointwise_relation _ (FreeTemps.t_eq ==> (⊢)) ==> (⊢))%signature.
 
+  Definition Mframe {T} (a b : M T) : mpred :=
+    Forall Q Q', (Forall x y, Q x y -* Q' x y) -* a Q -* b Q'.
+
   Definition Mret {T} (t : T) : M T :=
     fun K => K t FreeTemps.id.
 
   Definition Mmap {T U} (f : T -> U) (t : M T) : M U :=
     fun K => t (fun v => K (f v)).
 
+  Lemma Mmap_frame {T U} c (f : T -> U) :
+    Mframe c c |-- Mframe (Mmap f c) (Mmap f c).
+  Proof.
+    rewrite /Mframe/Mmap; iIntros "A" (??) "B".
+    iApply "A". iIntros (??); iApply "B".
+  Qed.
+
   Definition Mbind {T U} (c : M T) (k : T -> M U) : M U :=
     fun K => c (fun v f => k v (fun v' f' => K v' (f' >*> f)%free)).
+
+  Lemma Mbind_frame {T U} c (k : T -> M U) :
+    Mframe c c |-- (Forall x, Mframe (k x) (k x)) -* Mframe (Mbind c k) (Mbind c k).
+  Proof.
+    rewrite /Mframe/Mbind; iIntros "A B" (??) "C".
+    iApply "A". iIntros (??). iApply "B".
+    iIntros (??); iApply "C".
+  Qed.
 
   (** *** Indeterminately sequenced computations *)
   Definition nd_seq {T U} (wp1 : M T) (wp2 : M U) : M (T * U) :=
     fun K => wp1 (fun v1 f1 => wp2 (fun v2 f2 => K (v1,v2) (f2 >*> f1)%free))
      //\\ wp2 (fun v1 f1 => wp1 (fun v2 f2 => K (v2,v1) (f2 >*> f1)%free)).
+
+  Lemma nd_seq_frame {T U} wp1 wp2 :
+    Mframe wp1 wp1 |-- Mframe wp2 wp2 -* Mframe (@nd_seq T U wp1 wp2) (nd_seq wp1 wp2).
+  Proof.
+    iIntros "A B" (??) "C D".
+    iSplit; [ iDestruct "D" as "[D _]" | iDestruct "D" as "[_ D]" ]; iRevert "D".
+    { iApply "A". iIntros (??). iApply "B"; iIntros (??). iApply "C". }
+    { iApply "B". iIntros (??). iApply "A"; iIntros (??). iApply "C". }
+  Qed.
 
   (* unspecified sequencing of monadic compuations
      this is like the sematncis of argument evaluation in C++
@@ -295,8 +322,77 @@ Section with_cpp.
 
   Definition nd_seqs {T} qs := @nd_seqs' T (length qs) qs.
 
+  Lemma nd_seqs'_frame {T} n : forall (ls : list (M T)),
+      n = length ls ->
+      ([∗list] m ∈ ls, Mframe m m)
+      |-- Mframe (nd_seqs' n ls) (nd_seqs' n ls).
+  Proof.
+    induction n; simpl; intros.
+    { case_match.
+      { subst. simpl.
+        iIntros "_" (??) "X". iApply "X". }
+      { iIntros "?" (??) "? []". } }
+    { destruct ls. exfalso; simpl in *; congruence.
+      inversion H.
+      iIntros "LS" (??) "X Y"; iIntros (???) "%P".
+      iSpecialize ("Y" $! pre).
+      iSpecialize ("Y" $! post).
+      iSpecialize ("Y" $! q).
+      iDestruct ("Y" with "[]") as "Y"; first eauto.
+      rewrite P.
+      iDestruct "LS" as "(a&b&c)".
+      iRevert "Y".
+      iApply (Mbind_frame with "b [a c]"); eauto.
+      iIntros (?).
+      iApply Mmap_frame.
+      rewrite -H1.
+      iApply IHn.
+      { have: (length (m :: ls) = length (pre ++ q :: post)) by rewrite P.
+        rewrite !app_length /=. lia. }
+      iSplitL "a"; eauto. }
+  Qed.
+
+  Lemma nd_seqs_frame_strong {T} n : forall (ls : list (M T)) Q Q',
+      n = length ls ->
+      Forall x y, [| length x = length ls |] -* Q x y -* Q' x y
+      |-- ([∗list] m ∈ ls, Mframe m m) -*
+          nd_seqs' n ls Q -* nd_seqs' n ls Q'.
+  Proof.
+    induction n; simpl; intros.
+    { case_match; eauto.
+      subst. simpl.
+      iIntros "X _". iApply "X". eauto. }
+    { destruct ls. exfalso; simpl in *; congruence.
+      inversion H.
+      iIntros "X LS Y" (???) "%P".
+      iSpecialize ("Y" $! pre).
+      iSpecialize ("Y" $! post).
+      iSpecialize ("Y" $! q).
+      iDestruct ("Y" with "[]") as "Y"; first eauto.
+      rewrite P.
+      iDestruct "LS" as "(a&b&c)".
+      iRevert "Y". rewrite /Mbind.
+      iApply "b".
+      iIntros (??).
+      rewrite /Mmap.
+      subst.
+      assert (length ls = length (pre ++ post)).
+      { have: (length (m :: ls) = length (pre ++ q :: post)) by rewrite P.
+        rewrite !app_length /=. lia. }
+      iDestruct (IHn with "[X]") as "X". eassumption.
+      2:{
+      iDestruct ("X" with "[a c]") as "X".
+      iSplitL "a"; eauto.
+      iApply "X". }
+      simpl. iIntros (??) "%". iApply "X".
+      revert H0 H1. rewrite !app_length/=.
+      intros. iPureIntro.
+      rewrite firstn_length_le; last lia.
+      rewrite skipn_length. lia. }
+  Qed.
+
   (* sanity check on [nd_seq] and [nd_seqs] *)
-  Lemma nd_seq_ok : forall {T} (a b : M T),
+  Example nd_seq_example : forall {T} (a b : M T),
       Proper (Mrel _) a -> Proper (Mrel _) b ->
       Mrel _ (nd_seqs [a;b]) (Mmap (fun '(a,b) => [a;b]) $ nd_seq a b).
   Proof.
