theories/lang/cpp/logic/stmt.v
@@ -276,8 +276,8 @@ Module Type Stmt.
 
     Axiom wp_return : forall ρ e (Q : KpredI),
           (let rty := erase_qualifiers (get_return_type ρ) in
-           wp_call_initialize ρ rty e (fun v frees =>
-                                         interp frees (Q (ReturnVal v))))
+           Forall p, wp_initialize ρ rty p e (fun frees =>
+                                         interp frees (Q (ReturnVal p))))
            (* ^ NOTE discard [free] because we are extruding the scope of the value *)
        |-- wp ρ (Sreturn (Some e)) Q.
 
